src/Lean/Elab/Tactic/BVDecide/Frontend/BVDecide/Reflect.lean
@@ -44,7 +44,6 @@ instance : ToExpr BVUnOp where
     | .arithShiftRightConst n => mkApp (mkConst ``BVUnOp.arithShiftRightConst) (toExpr n)
     | .reverse => mkConst ``BVUnOp.reverse
     | .clz => mkConst ``BVUnOp.clz
-    | .cpop => mkConst ``BVUnOp.cpop
   toTypeExpr := mkConst ``BVUnOp
 
 instance : ToExpr (BVExpr w) where
@@ -72,6 +71,7 @@ where
     mkApp4 (mkConst ``BVExpr.shiftRight) (toExpr m) (toExpr n) (go lhs) (go rhs)
   | .arithShiftRight (m := m) (n := n) lhs rhs =>
     mkApp4 (mkConst ``BVExpr.arithShiftRight) (toExpr m) (toExpr n) (go lhs) (go rhs)
+  | .parPreSum (w := w) l expr => sorry
 
 instance : ToExpr BVBinPred where
   toExpr x :=
