src/Std/Tactic/BVDecide/Bitblast/BVExpr/Circuit/Impl/Expr.lean
@@ -232,12 +232,6 @@ where
           apply AIG.LawfulVecOperator.le_size_of_le_aig_size (f := bitblast.blastClz)
           omega
         ⟨⟨res, this⟩, cache.cast (AIG.LawfulVecOperator.le_size (f := bitblast.blastClz) ..)⟩
-      | .cpop =>
-        let res := bitblast.blastCpop eaig evec
-        have := by
-          apply AIG.LawfulVecOperator.le_size_of_le_aig_size (f := bitblast.blastCpop)
-          omega
-        ⟨⟨res, this⟩, cache.cast (AIG.LawfulVecOperator.le_size (f := bitblast.blastCpop) ..)⟩
     | .append lhs rhs h =>
       let ⟨⟨⟨aig, lhs⟩, hlaig⟩, cache⟩ := goCache aig lhs cache
       let ⟨⟨⟨aig, rhs⟩, hraig⟩, cache⟩ := goCache aig rhs cache
@@ -266,6 +260,7 @@ where
         dsimp only at heaig
         exact heaig
       ⟨⟨res, this⟩, cache.cast (AIG.LawfulVecOperator.le_size (f := bitblast.blastExtract) ..)⟩
+    | .parPreSum l expr => sorry
     | .shiftLeft lhs rhs =>
       let ⟨⟨⟨aig, lhs⟩, hlaig⟩, cache⟩ := goCache aig lhs cache
       let ⟨⟨⟨aig, rhs⟩, hraig⟩, cache⟩ := goCache aig rhs cache
@@ -349,7 +344,7 @@ theorem go_decl_eq (aig : AIG BVBit) (expr : BVExpr w) (cache : Cache aig) :
         · apply Nat.le_trans <;> assumption
   next op expr =>
     match op with
-    | .not | .rotateLeft .. | .rotateRight .. | .arithShiftRightConst .. | .reverse | .clz | .cpop =>
+    | .not | .rotateLeft .. | .rotateRight .. | .arithShiftRightConst .. | .reverse | .clz =>
       rw [AIG.LawfulVecOperator.decl_eq]
       rw [goCache_decl_eq]
       have := (goCache aig expr cache).result.property
@@ -373,6 +368,7 @@ theorem go_decl_eq (aig : AIG BVBit) (expr : BVExpr w) (cache : Cache aig) :
     rw [goCache_decl_eq]
     have := (goCache aig inner cache).result.property
     exact Nat.lt_of_lt_of_le h1 this
+  next _ _ => sorry
   next rhsExpr lhsExpr =>
     have hl := (goCache aig lhsExpr cache).result.property
     have hr := (goCache (goCache aig lhsExpr cache).1.1.aig rhsExpr (goCache aig lhsExpr cache).cache).result.property
